\documentclass{article}
\usepackage{mathtools}
\begin{document}
\begin{align}
  f &= 2xy + 3z \\
  f_1 &= 2 \\
  f_2 &= x && \frac{\partial f}{\partial f_2} = \frac{\partial f}{\partial f_3} \frac{\partial f_3}{\partial f_2} = d_3 d_{3,2}\\
  f_3 &= f_1 f_2 && \frac{\partial f}{\partial f_3} = d_3 = \frac{\partial f}{\partial f_5} \frac{\partial f_5}{\partial f_3} = d_5 d_{5,3} && \frac{\partial f_3}{\partial f_2} = d_{3,2} = f_1\\
  f_4 &= y \\
  f_5 &= f_3 f_4 && \frac{\partial f}{\partial f_5} = d_5 = \frac{\partial f}{\partial f_9} \frac{\partial f_9}{\partial f_5} = d_9 d_{9,5} && \frac{\partial f_5}{\partial f_3} = f_4\\
  f_6 &= 3\\
  f_7 &= z\\
  f_8 &= f_6 f_7 && \frac{\partial f}{\partial f_6} = \frac{\partial f}{\partial f_8} \frac{\partial f_8}{\partial f_6}\\
  f_9 &= f_5 + f_8 && \frac{\partial f}{\partial f_9} = d_9 = 1 && \frac{\partial f_9}{\partial f_5} = d_{9,5} = 1 && \frac{\partial f_9}{\partial f_8} = 1 \\
  \\
  \\
  f &= g(x,y)
\end{align}
\end{document}
